jelly_fish/rw_client/example.v
@@ -19,8 +19,6 @@ End Params.
 
 Module Import Spec := RWSpec Params.
 
-Definition exampleN := nroot .@ "example".
-
 Definition example_client : expr := 
   let: "p" := new #() in
     ((put "p" #10 #1 #0;; put "p" #20 #5 #1;; put "p" #10 #3 #2)
@@ -35,11 +33,11 @@ Section Proofs.
   Lemma example_client_spec :
     {{{ True }}}
       example_client
-    {{{ (v: Z), RET (SOMEV (#v, #2), SOMEV (#5, #1)); ⌜ v = 3 ∨ v = 4 ⌝ }}}.
+    {{{ v, RET (SOMEV (#v, #2), SOMEV (#5, #1)); ⌜ v = 3 ∨ v = 4 ⌝ }}}.
   Proof.
     iIntros (Φ) "_ HΦ"; unfold example_client.
-    wp_apply new_spec; first done. iIntros (p mΓ) "Hmap".
-    iDestruct (rw_inv_alloc_mut exampleN with "Hmap") as "Hinv".
+    wp_apply ts_new_spec; first done. iIntros (p mΓ) "Hmap".
+    iDestruct (rw_inv_alloc_mut with "Hmap") as "Hinv".
     iMod (fupd_mask_mono with "Hinv") as "Hinv"; first solve_ndisj.
     iDestruct "Hinv" as (Γ) "[#Hinv Hmut]".
 
@@ -47,35 +45,29 @@ Section Proofs.
     rewrite -(Qp.div_2 1); iDestruct (mut_map_sep with "Hmut") as "[Hmut1 Hmut2]".
     wp_smart_apply (wp_par (λ _, mut_map _ _ _) (λ _, mut_map _ _ _) with "[Hmut1] [Hmut2]").
     {
-      awp_apply (write_spec with "Hinv"); first rewrite /Params.INT_MIN/Params.INT_MAX//.
-      iAaccIntro with "Hmut1"; first (iIntros "?"; iModIntro; iFrame).
-      iIntros "Hmut1". iModIntro. iExists _. iFrame "Hmut1".
-      iIntros "Hmut1 _". iModIntro. wp_pures.
+      wp_apply (mut_spec with "Hinv Hmut1"); 
+        first rewrite /Params.INT_MIN/Params.INT_MAX//.
+      iIntros "Hmut1"; wp_pures.
 
-      awp_apply (write_spec with "Hinv"); first rewrite /Params.INT_MIN/Params.INT_MAX//.
-      iAaccIntro with "Hmut1"; first (iIntros "?"; iModIntro; iFrame).
-      iIntros "Hmut1". iModIntro. iExists _. iFrame "Hmut1".
-      iIntros "Hmut1 _". iModIntro. wp_pures.
+      wp_apply (mut_spec with "Hinv Hmut1"); 
+        first rewrite /Params.INT_MIN/Params.INT_MAX//.
+      iIntros "Hmut1"; wp_pures.
 
-      awp_apply (write_spec with "Hinv"); first rewrite /Params.INT_MIN/Params.INT_MAX//.
-      iAaccIntro with "Hmut1"; first (iIntros "?"; iModIntro; iFrame).
-      iIntros "Hmut1". iModIntro. iExists _. iFrame "Hmut1".
+      wp_apply (mut_spec with "Hinv Hmut1"); 
+        first rewrite /Params.INT_MIN/Params.INT_MAX//.
       by iIntros.
     }
     {
-      awp_apply (write_spec with "Hinv"); first rewrite /Params.INT_MIN/Params.INT_MAX//.
-      iAaccIntro with "Hmut2"; first (iIntros "?"; iModIntro; iFrame).
-      iIntros "Hmut2". iModIntro. iExists _. iFrame "Hmut2".
-      iIntros "Hmut2 _". iModIntro. wp_pures.
+      wp_apply (mut_spec with "Hinv Hmut2"); 
+        first rewrite /Params.INT_MIN/Params.INT_MAX//.
+      iIntros "Hmut2"; wp_pures.
 
-      awp_apply (write_spec with "Hinv"); first rewrite /Params.INT_MIN/Params.INT_MAX//.
-      iAaccIntro with "Hmut2"; first (iIntros "?"; iModIntro; iFrame).
-      iIntros "Hmut2". iModIntro. iExists _. iFrame "Hmut2".
-      iIntros "Hmut2 _". iModIntro. wp_pures.
+      wp_apply (mut_spec with "Hinv Hmut2"); 
+        first rewrite /Params.INT_MIN/Params.INT_MAX//.
+      iIntros "Hmut2"; wp_pures.
 
-      awp_apply (write_spec with "Hinv"); first rewrite /Params.INT_MIN/Params.INT_MAX//.
-      iAaccIntro with "Hmut2"; first (iIntros "?"; iModIntro; iFrame).
-      iIntros "Hmut2". iModIntro. iExists _. iFrame "Hmut2".
+      wp_apply (mut_spec with "Hinv Hmut2"); 
+        first rewrite /Params.INT_MIN/Params.INT_MAX//.
       by iIntros.
     }
     iIntros (? ?) "Hmut". rewrite ?left_id_L.
@@ -90,19 +82,19 @@ Section Proofs.
       (λ v, ⌜ v = SOMEV (#5, #1) ⌝%I)
     with "[Hconst1] [Hconst2]").
     {
-      awp_apply (read_spec with "Hinv"); first rewrite /Params.INT_MIN/Params.INT_MAX//.
-      iAaccIntro with "Hconst1"; first (iIntros "?"; iModIntro; iFrame).
-      iIntros (opt) "Hconst1". iModIntro. iExists _. iFrame "Hconst1". iIntros "_ Hopt".
-      iDestruct "Hopt" as (vs v t) "(%Hprod & %Hin & %Hopt)". iPureIntro.
+      wp_apply (const_spec with "Hinv Hconst1");
+        first rewrite /Params.INT_MIN/Params.INT_MAX//.
+      iIntros (opt) "[Hconst1 %Hopt]". iPureIntro.
+      destruct Hopt as (vs & v & t & Hprod & Hin & Hopt).
       rewrite argmax_eq in Hprod; inversion Hprod; subst.
       rewrite elem_of_union ?elem_of_singleton in Hin.
       destruct Hin; subst; first (by left); last (by right).
     }
     {
-      awp_apply (read_spec with "Hinv"); first rewrite /Params.INT_MIN/Params.INT_MAX//.
-      iAaccIntro with "Hconst2"; first (iIntros "?"; iModIntro; iFrame).
-      iIntros (opt) "Hconst2". iModIntro. iExists _. iFrame "Hconst2". iIntros "_ Hopt".
-      iDestruct "Hopt" as (vs v t) "(%Hprod & %Hin & %Hopt)". iPureIntro.
+      wp_apply (const_spec with "Hinv Hconst2");
+        first rewrite /Params.INT_MIN/Params.INT_MAX//.
+      iIntros (opt) "[Hconst2 %Hopt]". iPureIntro.
+      destruct Hopt as (vs & v & t & Hprod & Hin & Hopt).
       rewrite comm_L argmax_lt // in Hprod; inversion Hprod; subst.
       rewrite elem_of_singleton in Hin; by subst.
     }
